Fix mistake in spin-lock and add description

solutions/spin_lock.v
@@ -2,14 +2,33 @@ From iris.algebra Require Import excl.
 From iris.base_logic.lib Require Export invariants.
 From iris.heap_lang Require Import lang proofmode notation.
 
+(*
+  A spin-lock consists of a pointer to a boolean. This boolean tells us
+  whether the lock is currently locked or not.
+
+  To make a new lock, we simply allocate a new boolean.
+*)
 Definition mk_lock : val :=
   λ: <>, ref #false.
+
+(*
+  To acquire the lock, we use `CAS l false true` (compare and set).
+  This is an atomic operation that updated l to true if l was false.
+  `CAS` then evaluates to whether l was updated.
+  If the CAS fails, it means that the lock is currently acquired
+  somewhere else. So we simply again, until the lock is free.
+*)
 Definition acquire : val :=
   rec: "acquire" "l" :=
   if: CAS "l" #false #true then
     #()
   else
     "acquire" "l".
+
+(*
+  To release a lock, we simply update the boolean to false. As such
+  it is only safe to call release when we are the ones who locked it.
+*)
 Definition release : val :=
   λ: "l", "l" <- #false.
 
@@ -17,16 +36,50 @@ Section proofs.
 Context `{heapGS Σ}.
 Let N := nroot .@ "lock".
 
-Context `{inG Σ (excl ())}.
+(*
+  We use ghost state to describe that the lock is only ever acquired
+  once at a time. To do this we simply need ghost state that is
+  exclusive. So naturally we will use the exclusive camera. This
+  camera is generic over state, however we don't need this feature. So
+  we will instatiate it with unit.
+*)
+Context `{!inG Σ (excl ())}.
 
-Definition locked γ : iProp Σ := own γ (Excl ()).
-
+(*
+  We will think of the name of our ghost state as the name of the
+  lock. It's invariant will be that l maps to a boolean b, and if
+  b is false, meaning the lock is unlocked, then the invariant owns
+  both the resource and the critical area protected by the lock.
+*)
 Definition lock_inv γ l P : iProp Σ :=
-  ∃ b : bool, l ↦ #b ∗ if b then True else own γ (Excl ()) ∗ P.
+  ∃ b : bool, l ↦ #b ∗
+  if b then True
+  else own γ (Excl ()) ∗ P.
 
 Definition is_lock γ v P : iProp Σ :=
   ∃ l : loc, ⌜v = #l⌝ ∗ inv N (lock_inv γ l P).
 
+(*
+  The knowledge that we have acquired the is then represented by
+  ownership of the resource.
+*)
+Definition locked γ : iProp Σ := own γ (Excl ()).
+
+(*
+  We need the ghost state to prove that this is exclusive.
+*)
+Lemma locked_excl γ : locked γ -∗ locked γ -∗ False.
+Proof.
+  iIntros "H1 H2".
+  iPoseProof (own_valid_2 with "H1 H2") as "%H".
+  cbv in H.
+  done.
+Qed.
+
+(*
+  Making a new lock consists of giving away ownership of the critical
+  area to the lock.
+*)
 Lemma mk_lock_spec P : {{{ P }}} mk_lock #() {{{ γ v, RET v; is_lock γ v P }}}.
 Proof.
   iIntros "%Φ HP HΦ".
@@ -46,7 +99,11 @@ Proof.
   by iFrame.
 Qed.
 
-Lemma acquire_spec γ v P : {{{ is_lock γ v P }}} acquire v {{{ γ v, RET v; locked γ ∗ P }}}.
+(*
+  Acquirering the lock should result in access to the critical area,
+  as well as knowledge that the lock has been locked.
+*)
+Lemma acquire_spec γ v P : {{{ is_lock γ v P }}} acquire v {{{ RET #(); locked γ ∗ P }}}.
 Proof.
   iIntros "%Φ (%l & -> & #I) HΦ".
   iLöb as "IH".
@@ -88,6 +145,53 @@ Proof.
     iExists false.
     iFrame.
   - by iApply "HΦ".
+Qed.
+
+Definition prog : expr :=
+  let: "x" := ref #0 in
+  let: "l" := mk_lock #() in
+  Fork (
+    acquire "l";;
+    "x" <- #7;;
+    "x" <- #1;;
+    release "l"
+  );;
+  acquire "l";;
+  !"x".
+
+(*
+  x can take on the values of 0, 1, and 7. However we should not
+  observe 7, as it is overriden before the lock is released.
+*)
+Lemma prog_spec : ⊢ WP prog {{ v, ⌜v = #0 ∨ v = #1⌝}}.
+Proof.
+  rewrite /prog.
+  wp_alloc x as "Hx".
+  wp_pures.
+  wp_apply (mk_lock_spec (∃ v, x ↦ v ∗ ⌜v = #0 ∨ v = #1⌝) with "[Hx]").
+  {
+    iExists #0.
+    iFrame.
+    by iLeft.
+  }
+  iIntros "%γ %l #Hl".
+  wp_pures.
+  wp_apply wp_fork.
+  - wp_apply (acquire_spec with "Hl").
+    iIntros "(H & %v & Hx & _)".
+    wp_pures.
+    wp_store.
+    wp_store.
+    wp_apply (release_spec with "[$Hl $H Hx]"); last done.
+    iExists #1.
+    iFrame.
+    by iRight.
+  - wp_pures.
+    wp_apply (acquire_spec with "Hl").
+    iIntros "(_ & %v & Hx & Hv)".
+    wp_pures.
+    wp_load.
+    done.
 Qed.
 
 End proofs.
